added a preservation and progress based proof method of lts_safe; removed old definitions of lts_safe and its compositionality proof

common/SmallstepLinkingSafe.v
@@ -83,32 +83,131 @@ Record lts_safe {liA liB S} se (L: lts liA liB S) (IA: invariant liA) (IB: invar
     final_progress: forall s r,
       reachable IA IB L wI s ->
       final_state L s r ->
-      reply_inv IB wI r;
-    
+      reply_inv IB wI r;    
   }.
+
+Definition module_safe_se {liA liB} (L: semantics liA liB) (IA IB: invariant _) SI se :=
+  forall w,
+    symtbl_inv IB w se ->
+    lts_safe se (L se) IA IB SI w.
+
+Definition module_safe {liA liB} (L: semantics liA liB) (IA IB: invariant _) SI :=
+  forall se,
+    Genv.valid_for (skel L) se ->
+    module_safe_se L IA IB SI se.
 
 (** Proof of lts_safe by the method of preservation and progress *)
 
-(* Record invariant_preserves {liA liB S} se (L: lts liA liB S) (IA: invariant liA) (IB: invariant liB) (IS: _ -> S -> Prop) (wI: inv_world IB) := *)
-(*   { *)
-(*     initial_preserves: forall q s, *)
-(*       query_inv IB wI q -> *)
-(*       initial_state L q s -> *)
-(*       IS wI s; *)
+(* silightly different from lts_preserves in Invariant.v *)
+Record lts_invariant_preserves {liA liB S} (L: lts liA liB S) (IA: invariant liA) (IB: invariant liB) (IS: inv_world IB -> S -> Prop) (w: inv_world IB) :=
+  {
+    preserves_step s t s':
+      IS w s ->
+      Step L s t s' ->
+      IS w s';
+    preserves_initial_state q s:
+      (* valid_query L q = true -> *)
+      query_inv IB w q ->
+      initial_state L q s ->
+      IS w s;
+    (** Why? *)
+    preserves_external s s' q r wA:
+      IS w s ->
+      at_external L s q ->
+      query_inv IA wA q ->
+      reply_inv IA wA r ->
+      after_external L s r s' ->
+      IS w s';
+  }.
 
-(*     step_preserves: forall s t s', *)
-(*       IS wI s -> *)
-      
-      
-(*   } . *)
+(* not_stuck is hard code in lts_invariant_progress *)
+Record lts_invariant_progress {liA liB S} se (L: lts liA liB S) (IA: invariant liA) (IB: invariant liB) (IS: inv_world IB -> S -> Prop) (w: inv_world IB) :=
+  {
+    progress_internal_state: forall s,
+      IS w s ->
+      not_stuck L s;
+
+    progress_initial_state: forall q,
+      valid_query L q = true ->
+      query_inv IB w q ->
+      (exists s, initial_state L q s);
+    
+    progress_external_state: forall s q,
+      IS w s ->
+      at_external L s q ->
+      exists wA, symtbl_inv IA wA se /\ query_inv IA wA q /\
+              forall r, reply_inv IA wA r ->
+                   (* after external progress *)
+                   (exists s', after_external L s r s');
+
+    progress_final_state: forall s r,
+      IS w s ->
+      final_state L s r ->
+      reply_inv IB w r;
+  }.
 
 
-(** Proof of compositionality of module safe *)
-Definition module_safe {liA liB} (L: semantics liA liB) (IA IB: invariant _) SI se :=
-  forall w,
-    Genv.valid_for (skel L) se ->
-    symtbl_inv IB w se ->
-    lts_safe se (L se) IA IB SI w.
+Record module_safe_components {liA liB} (L: semantics liA liB) (IA: invariant liA) (IB: invariant liB) :=
+  {
+    msafe_invariant: inv_world IB -> state L -> Prop;
+
+    msafe_preservation: forall se wB,
+      symtbl_inv IB wB se ->
+      Genv.valid_for (skel L) se ->
+      lts_invariant_preserves (L se) IA IB msafe_invariant wB;
+
+    msafe_progress: forall se wB,
+      symtbl_inv IB wB se ->
+      Genv.valid_for (skel L) se ->
+      lts_invariant_progress se (L se) IA IB msafe_invariant wB;
+  }.
+
+Lemma star_preserves_invariant {liA liB S} (L: lts liA liB S) (IA: invariant liA) (IB: invariant liB): forall w s t s' IS (PRE: lts_invariant_preserves L IA IB IS w),
+    IS w s ->
+    Star L s t s' ->
+    IS w s'.
+Proof.
+  induction 3. auto.
+  apply IHstar. eapply preserves_step; eauto.
+Qed.
+
+Lemma reachable_preserves_invariant {liA liB S} (L: lts liA liB S) (IA: invariant liA) (IB: invariant liB): forall w s IS (PRE: lts_invariant_preserves L IA IB IS w),
+    reachable IA IB L w s ->
+    IS w s.
+Proof.
+  induction 2.
+  - eapply star_preserves_invariant; eauto.
+    eapply preserves_initial_state; eauto.
+  - eapply star_preserves_invariant. 3: eapply STEP. eauto.
+    eapply preserves_external; eauto.
+Qed.
+
+(* soundness of module_safe_components *)
+Lemma module_safe_components_sound {liA liB} (L: semantics liA liB) (IA: invariant liA) (IB: invariant liB):
+  module_safe_components L IA IB ->
+  module_safe L IA IB not_stuck.
+Proof.
+  intros SAFE. inv SAFE.
+  red. intros se VSE w WTSE.
+  exploit msafe_preservation0; eauto. intros PRE.
+  exploit msafe_progress0; eauto. intros PRO.
+  constructor.
+  (* reachable not stuck *)
+  - intros s REACH.
+    eapply reachable_preserves_invariant with (IS:= msafe_invariant0) in REACH; auto.
+    eapply progress_internal_state; eauto.
+  (* initial_progress *)
+  - eapply progress_initial_state; eauto.
+  (* external_progress *)
+  - intros s q REACH.
+    eapply progress_external_state; eauto.
+    eapply reachable_preserves_invariant; eauto.
+  (* final_progress *)
+  - intros s r REACH.
+    eapply progress_final_state; eauto.
+    eapply reachable_preserves_invariant; eauto.
+Qed.
+
 
 (* Propeties of reachable state in composed semantics *)
 Section REACH.
@@ -143,7 +242,7 @@ Inductive wf_state : list (frame L) -> Prop :=
 Section SAFE.
 
 Hypothesis (VALIDSE: forall i, Genv.valid_for (skel (L i)) se).
-Hypothesis (SAFE: forall i, module_safe (L i) I I not_stuck se).
+Hypothesis (SAFE: forall i, module_safe_se (L i) I I not_stuck se).
 
 Lemma step_wf_state sk s1 t s2:
   Step (SmallstepLinking.semantics L sk se) s1 t s2 ->
@@ -205,24 +304,27 @@ End SAFE.
 
 End REACH.
 
-Lemma compose_safety {li} (I: invariant li) L1 L2 L se:
-  module_safe L1 I I not_stuck se ->
-  module_safe L2 I I not_stuck se ->
+(** Proof of compositionality of module safe *)
+
+Lemma compose_safety {li} (I: invariant li) L1 L2 L:
+  module_safe L1 I I not_stuck ->
+  module_safe L2 I I not_stuck ->
   compose L1 L2 = Some L ->
-  module_safe L I I not_stuck se.
+  module_safe L I I not_stuck.
 Proof.
   intros SAFE1 SAFE2 COMP. unfold compose in *. unfold option_map in *.
   destruct (link (skel L1) (skel L2)) as [sk|] eqn:Hsk; try discriminate. inv COMP.
   set (L := fun i:bool => if i then L1 else L2).
-  red. intros w VALID INV.
+  red. intros se w VALID INV.
   assert (VALIDSE: forall i, Genv.valid_for (skel (L i)) se).
   destruct i.
   eapply Genv.valid_for_linkorder.
   eapply (link_linkorder _ _ _ Hsk). eauto.
   eapply Genv.valid_for_linkorder.
   eapply (link_linkorder _ _ _ Hsk). eauto.
-  assert (SAFE: forall i, module_safe (L i) I I not_stuck se).
-  destruct i; simpl; auto.
+  assert (SAFE: forall i, module_safe_se (L i) I I not_stuck se).
+  { intros i. generalize (VALIDSE i). intros VSE.
+    destruct i; simpl; auto. }
   constructor.
   (* rechable not stuck *)
   - intros s WFREACH.    
@@ -245,7 +347,7 @@ Proof.
       * red. right. right.
         inv WFS.
         (* final_prgress in s0 *)
-        exploit (@final_progress li). eapply SAFE. eapply VALIDSE.
+        exploit (@final_progress li). eapply SAFE.
         eapply VSE. eauto. eauto. intros WTR.        
         exploit PGS; eauto. intros (s1' & AFEXT).
         (* s0 can return a well-typed reply to s1 which is in at_external to make a step *)
@@ -308,224 +410,8 @@ Proof.
 Qed.
 
 
-(** Remove the following code (old lts_safe) *)
-(* (** TODO: generalize safe/partial_safe to module linking and show that *)
-(* the original safe/partial_safe is identical to the composed *)
-(* safe/partial_safe *) *)
-
-(* (** TODO: essence behind the rechable predicate? i.e., how to prove *)
-(* lts_safe using lts_preserve in Invariant.v. TODO: try to define a *)
-(* proper rechable predicate to prove that lts_preserve /\ rechable -> *)
-(* sound_state *) *)
-(* Record lts_safe {liA liB S} se (L: lts liA liB S) (IA: invariant liA) (IB: invariant liB) (SI: _ -> S -> Prop) (wI: inv_world IB) := *)
-(*   { *)
-(*     step_safe s t s' (REACH: reachable L s): *)
-(*     (* SI may be stronger than safe, but how to preserve the stronger part *) *)
-(*       (* SI L s -> *) *)
-(*       Step L s t s' -> *)
-(*       SI L s'; *)
-(*     initial_safe q: *)
-(*       valid_query L q = true -> *)
-(*       query_inv IB wI q -> *)
-(*       (* initial_progress *) *)
-(*       (exists s, initial_state L q s) *)
-(*       (* initial_safe *) *)
-(*       /\ (forall s, initial_state L q s -> SI L s); *)
-(*     external_safe s q (REACH: reachable L s): *)
-(*       at_external L s q -> *)
-(*       exists wA, symtbl_inv IA wA se /\ query_inv IA wA q /\ *)
-(*               forall r, reply_inv IA wA r -> *)
-(*                    (* after external progress *) *)
-(*                    (exists s', after_external L s r s') *)
-(*                    (* after external safe *) *)
-(*                    /\ (forall s', after_external L s r s' -> SI L s'); *)
-(*     final_safe s r (REACH: reachable L s): *)
-(*       final_state L s r -> *)
-(*       reply_inv IB wI r; *)
-(*   }. *)
-
-
-(* (* se as an oracle, is it correct? *) *)
-(* Definition module_safe {liA liB} (L: semantics liA liB) (IA IB: invariant _) SI se := *)
-(*   forall w, *)
-(*     Genv.valid_for (skel L) se -> *)
-(*     symtbl_inv IB w se -> *)
-(*     lts_safe se (L se) IA IB SI w. *)
-
-
-(* Lemma safe_internal {li} (I: invariant li) L1 L2: forall i sk se s k w, *)
-(*     let L := fun (i:bool) => if i then L1 else L2 in *)
-(*     forall (Hsk: link (skel L1) (skel L2) = Some sk) *)
-(*       (VALID: Genv.valid_for (skel (SmallstepLinking.semantics L sk)) se) *)
-(*       (INV : symtbl_inv I w se) *)
-(*       (VALIDSE: forall i, Genv.valid_for (skel (L i)) se) *)
-(*       (SAFE: forall i, module_safe (L i) I I safe se) *)
-(*       (STSAFE: safe (L i se) s) *)
-(*       (WFSTATE: wf_state L se (st L i s :: k)), *)
-(*       safe (SmallstepLinking.semantics L sk se) (st L i s :: k). *)
-(* Proof. *)
-(*   intros. *)
-(*   destruct STSAFE as [(r & FINAL)|[(q & EXT)|(t1 & s1 & STEP1)]]. *)
-(*   * destruct k. *)
-(*     -- left. exists r. *)
-(*        econstructor. auto. *)
-(*     -- destruct f. *)
-(*        right. right. *)
-(*        (* s0 in in at_external state *) *)
-(*        inv WFSTATE. subst_dep. inv H3. inv H2. subst_dep. *)
-(*        generalize (external_safe _ _ _ _ _ _ (SAFE i0 _ (VALIDSE i0) INV) s0 q H5 H3). *)
-(*        intros (wA & SYMBINV & QINV & AFTER). *)
-(*        generalize (final_safe _ _ _ _ _ _ (SAFE i _ (VALIDSE i) SYMBINV) _ _ H1 FINAL). *)
-(*        intros WR. *)
-(*        generalize (AFTER _ WR). *)
-(*        intros ((s0' & AFTER1) & SAFTER). *)
-(*        do 2 eexists. *)
-(*        eapply step_pop; eauto. *)
-(*   * inv WFSTATE. subst_dep. *)
-(*     generalize (external_safe _ _ _ _ _ _ (SAFE i _ (VALIDSE i) INV) s q H1 EXT). *)
-(*     intros (wA & SYMBINV & QINV & AFTER). *)
-(*     destruct (valid_query (L i se) q) eqn: VQ1. *)
-(*     -- right. right. *)
-(*        generalize (initial_safe _ _ _ _ _ _ (SAFE i _ (VALIDSE i) SYMBINV) _ VQ1 QINV). *)
-(*        intros ((initS & INIT) & INITSAFE). *)
-(*        do 2 eexists. *)
-(*        eapply step_push; eauto. *)
-(*     -- destruct i; simpl in *. *)
-(*        ++ destruct (valid_query (L2 se) q) eqn: VQ2. *)
-(*           ** right. right. *)
-(*              generalize (initial_safe _ _ _ _ _ _ (SAFE false _ (VALIDSE false) SYMBINV) _ VQ2 QINV). *)
-(*              intros ((initS & INIT) & INITSAFE). *)
-(*              do 2 eexists. *)
-(*              eapply step_push. eauto. *)
-(*              instantiate (1 := false). auto. *)
-(*              simpl. eauto. *)
-(*           ** right. left. *)
-(*              eexists. econstructor. *)
-(*              simpl. eauto. *)
-(*              intros. destruct j; simpl; auto. *)
-(*        ++  destruct (valid_query (L1 se) q) eqn: VQ2. *)
-(*            ** right. right. *)
-(*               generalize (initial_safe _ _ _ _ _ _ (SAFE true _ (VALIDSE true) SYMBINV) _ VQ2 QINV). *)
-(*               intros ((initS & INIT) & INITSAFE). *)
-(*               do 2 eexists. *)
-(*               eapply step_push. eauto. *)
-(*               instantiate (1 := true). auto. *)
-(*               simpl. eauto. *)
-(*            ** right. left. *)
-(*               eexists. econstructor. *)
-(*               simpl. eauto. *)
-(*               intros. destruct j; simpl; auto. *)
-(*   * right. right. do 2 eexists. *)
-(*     eapply step_internal. simpl. eauto. *)
-(* Qed. *)
-
-
-(* Lemma compose_safety {li} (I: invariant li) L1 L2 L se: *)
-(*   module_safe L1 I I safe se -> *)
-(*   module_safe L2 I I safe se -> *)
-(*   compose L1 L2 = Some L -> *)
-(*   module_safe L I I safe se. *)
-(* Proof. *)
-(*   intros SAFE1 SAFE2 COMP. unfold compose in *. unfold option_map in *. *)
-(*   destruct (link (skel L1) (skel L2)) as [sk|] eqn:Hsk; try discriminate. inv COMP. *)
-(*   set (L := fun i:bool => if i then L1 else L2). *)
-(*   red. intros w VALID INV. *)
-(*   assert (VALIDSE: forall i, Genv.valid_for (skel (L i)) se). *)
-(*   destruct i. *)
-(*   eapply Genv.valid_for_linkorder. *)
-(*   eapply (link_linkorder _ _ _ Hsk). eauto. *)
-(*   eapply Genv.valid_for_linkorder. *)
-(*   eapply (link_linkorder _ _ _ Hsk). eauto. *)
-(*   assert (SAFE: forall i, module_safe (L i) I I safe se). *)
-(*   destruct i; simpl; auto. *)
-(*   constructor. *)
-(*   - intros s t s' REACH STEP. *)
-(*     eapply reachable_wf_state in REACH. *)
-(*     inv STEP. *)
-(*     + (* destruct i; simpl in H. *) *)
-(*       assert (A: safe (L i se) s0). right. right. eauto. *)
-(*       assert (B: safe (L i se) s'0). { *)
-(*         eapply step_safe; eauto. eapply SAFE; eauto. *)
-(*         inv REACH. subst_dep. auto. } *)
-(*       eapply safe_internal; eauto. *)
-(*       inv REACH. subst_dep. econstructor;eauto. eapply step_reachable; eauto. *)
-(*     (* step_push *) *)
-(*     + assert (A: safe (L i se) s0). right. left. eauto. *)
-(*       assert (B: safe (L j se) s'0). *)
-(*       { inv REACH. subst_dep. *)
-(*         generalize (external_safe _ _ _ _ _ _ (SAFE i _ (VALIDSE i) INV) s0 q H4 H). *)
-(*         intros (wA & SYMBINV & QINV & AFTER). *)
-(*         eapply initial_safe. eapply SAFE; eauto. eauto. auto. auto. } *)
-(*       eapply safe_internal;eauto. *)
-(*       constructor; eauto. econstructor; eauto. *)
-(*       eapply star_refl. *)
-(*       inv REACH. subst_dep. econstructor;eauto. *)
-(*       econstructor;eauto. *)
-(*     (* step_pop *) *)
-(*     + inv REACH. inv H5. subst_dep. *)
-(*       inv H6. subst_dep. *)
-(*       assert (ATEXT: exists q, at_external (L j se) sk0 q). *)
-(*       eauto. *)
-(*       destruct ATEXT as (q1 & ATEXT). *)
-(*       generalize (external_safe _ _ _ _ _ _ (SAFE j _ (VALIDSE j) INV) sk0 q1 H5 ATEXT). *)
-(*       intros (wA & SYMBINV & QINV & AFTER). *)
-(*       generalize (final_safe _ _ _ _ _ _ (SAFE i _ (VALIDSE i) SYMBINV) _ _ H3 H). *)
-(*       intros VR. *)
-(*       generalize (AFTER r VR). *)
-(*       intros ((s' & AFTER1) & C). *)
-(*       assert (B: safe (L j se) s'0). eapply C. eauto. *)
-(*       eapply safe_internal; eauto. *)
-(*       econstructor;eauto. eapply external_reach. eapply H5. eapply H0. *)
-(*       eapply star_refl. *)
-(*   (* initial_safe *) *)
-(*   - intros q VQ SQ. simpl in *. *)
-(*     unfold SmallstepLinking.valid_query in VQ. *)
-(*     simpl in *. split. *)
-(*     + (* progress *) *)
-(*       destruct (valid_query (L1 se) q) eqn: VQ1. *)
-(*       * generalize (initial_safe _ _ _ _ _ _ (SAFE true _ (VALIDSE true) INV) _ VQ1 SQ). *)
-(*         intros ((s & INIT) & INITSAFE). *)
-(*         exists (st L true s :: nil). econstructor; eauto. *)
-(*       * rewrite orb_false_l in VQ. *)
-(*         generalize (initial_safe _ _ _ _ _ _ (SAFE false _ (VALIDSE false) INV) _ VQ SQ). *)
-(*         intros ((s & INIT) & INITSAFE). *)
-(*         exists (st L false s :: nil). econstructor; eauto. *)
-(*     + (* safe *) *)
-(*       intros s INIT. *)
-(*       inv INIT. *)
-(*       generalize (initial_safe _ _ _ _ _ _ (SAFE i _ (VALIDSE i) INV) _ H SQ). *)
-(*       intros ((s & INIT) & INITSAFE). *)
-(*       (* repeated work *) *)
-(*       clear INIT. *)
-(*       eapply safe_internal; eauto. *)
-(*       econstructor. eapply initial_reach; eauto. *)
-(*       eapply star_refl. constructor.   *)
-(*   - intros s q REACH EXT. inv EXT. *)
-(*     eapply reachable_wf_state in REACH. inv REACH. subst_dep. *)
-(*     generalize (external_safe _ _ _ _ _ _ (SAFE i _ (VALIDSE i) INV) s0 q H3 H). *)
-(*     intros (wA & SYMBINV & QINV & AFTER). *)
-(*     exists wA. split; auto. split; auto. *)
-(*     intros r SR. *)
-(*     generalize (AFTER r SR). *)
-(*     intros ((s' & AFTER1) & C). *)
-(*     split. exists (st L i s' :: k). econstructor; eauto. *)
-(*     intros s1' AFTER2. simpl in *. inv AFTER2.  *)
-(*     subst_dep. *)
-(*     generalize (C s'0 H8). intros D. *)
-(*     (* repeated work *) *)
-(*     eapply safe_internal; eauto. *)
-(*     econstructor; eauto. eapply external_reach; eauto. *)
-(*     eapply star_refl.     *)
-(*   - intros s r REACH FINAL. *)
-(*     inv FINAL. *)
-(*     apply reachable_wf_state in REACH. inv REACH. subst_dep. *)
-(*     generalize (final_safe _ _ _ _ _ _ (SAFE i _ (VALIDSE i) INV) _ _ H2 H). *)
-(*     auto. *)
-(* Qed. *)
-
-
 (* similar to ccref *)
-Record bsim_invariant_new {li1 li2} (cc: callconv li1 li2) (I1: invariant li1) (I2: invariant li2) : Type :=
+Record bsim_invariant {li1 li2} (cc: callconv li1 li2) (I1: invariant li1) (I2: invariant li2) : Type :=
   {
     (* incoming_query2 and outgoing_query2 are used to establish
     match_states between rechable states *)
@@ -565,99 +451,6 @@ Record bsim_invariant_new {li1 li2} (cc: callconv li1 li2) (I1: invariant li1) (
   }.
 
 
-(* Relation between two semantics invariants *)
-(* Record bsim_invariant {li1 li2} (cc: callconv li1 li2) (I1: invariant li1) (I2: invariant li2) : Type := *)
-(*   { inv_match_world: ccworld cc -> inv_world I1 -> inv_world I2 -> Prop; *)
-
-(*     (** TODO: how to get inv_match_world? *) *)
-(*     inv_match_symtbl: forall w2 se1 se2 ccw, *)
-(*       symtbl_inv I2 w2 se2 -> *)
-(*       match_senv cc ccw se1 se2 -> *)
-(*       exists w1, inv_match_world ccw w1 w2 *)
-(*             /\ symtbl_inv I1 w1 se1; *)
-
-(*     inv_match_query: forall w1 w2 q2 ccw, *)
-(*       query_inv I2 w2 q2 -> *)
-(*       inv_match_world ccw w1 w2 -> *)
-(*       exists q1, match_query cc ccw q1 q2 *)
-(*             /\ query_inv I1 w1 q1; *)
-
-(*     inv_match_reply: forall w1 w2 r2 ccw, *)
-(*       reply_inv I2 w2 r2 -> *)
-(*       inv_match_world ccw w1 w2 -> *)
-(*       exists r1, match_reply cc ccw r1 r2 *)
-(*             /\ reply_inv I1 w1 r1 *)
-
-(*   }. *)
-
-(* Section LTS_SAFETY_PRESERVATION. *)
-
-(* Context {li1 li2} (cc: callconv li1 li2). *)
-(* Context {state1 state2: Type}. *)
-(* Context (L1: lts li1 li1 state1) (L2: lts li2 li2 state2). *)
-(* Context (I1: invariant li1) (I2: invariant li2). *)
-(* Context (se1 se2: Genv.symtbl). *)
-(* Context (ccw: ccworld cc) (w1: inv_world I1) (w2: inv_world I2). *)
-(* Context {index: Type} (order: index -> index -> Prop). *)
-(* Context (match_states: index -> state1 -> state2 -> Prop). *)
-
-(* Hypothesis BSIM_INV: bsim_invariant cc I1 I2. *)
-(* Hypothesis MATCHWORLD: inv_match_world cc I1 I2 BSIM_INV ccw w1 w2. *)
-
-(* Lemma lts_safety_preservation: *)
-(*   lts_safe se1 L1 I1 I1 safe w1 -> *)
-(*   bsim_properties cc cc se1 se2 ccw L1 L2 index order match_states -> *)
-(*   lts_safe se2 L2 I2 I2 safe w2. *)
-(* Proof. *)
-(*   intros SAFE1 BSIM. *)
-(*   inv BSIM. inv SAFE1. *)
-(*   econstructor. *)
-(*   (* prove lts safety preservation *) *)
-(*   econstructor. *)
-(*   (* step_safe *) *)
-(*   - admit. *)
-(*   (* initial_safe *) *)
-(*   - intros q2 QV2 QINV2. *)
-(*     generalize (inv_match_query _ _ _ BSIM_INV w1 w2 q2 ccw QINV2 MATCHWORLD). *)
-(*     intros (q1 & MQ & QINV1). *)
-(*     exploit initial_safe0. *)
-(*     erewrite <- bsim_match_valid_query; eauto. *)
-(*     auto. admit. *)
-    
-(*   (* external_safe *) *)
-(*   - admit. *)
-(*   (* final_safe *) *)
-(*   - admit. *)
-(* Admitted. *)
-
-
-(* End LTS_SAFETY_PRESERVATION. *)
-
-Record bsim_invariant {li1 li2} (cc: callconv li1 li2) (I1: invariant li1) (I2: invariant li2) : Type :=
-  { inv_initial: forall w2 se1 se2 ccw q2, 
-      symtbl_inv I2 w2 se2 ->
-      match_senv cc ccw se1 se2 ->
-      query_inv I2 w2 q2 ->
-      exists w1 q1, symtbl_inv I1 w1 se1
-               /\ query_inv I1 w1 q1
-               (* used to establish simulation in initial states *)
-               /\ match_query cc ccw q1 q2;
-    inv_external: forall w1 se1 se2 ccw q1 q2, 
-      symtbl_inv I1 w1 se1 ->
-      match_senv cc ccw se1 se2 ->
-      query_inv I1 w1 q1 ->
-      match_query cc ccw q1 q2 ->
-      exists w2, symtbl_inv I2 w2 se2
-            /\ query_inv I2 w2 q2
-            /\ (forall r2, reply_inv I2 w2 r2 ->
-                     exists r1, reply_inv I1 w1 r1
-                           /\ match_reply cc ccw r1 r2);
-    inv_final: forall w1 ccw r1 r2, 
-      reply_inv I1 w1 r1 ->
-      match_reply cc ccw r1 r2 ->
-      exists w2, reply_inv I2 w2 r2;
-}.
-
 
 (** Safety Preservation Under Backward Simulation *)
 
@@ -672,53 +465,53 @@ Hypothesis BSIM_INV: bsim_invariant cc I1 I2.
 
 Lemma module_safety_preservation:
   match_senv cc ccw se1 se2 ->
-  module_safe L1 I1 I1 safe se1 ->
+  module_safe_se L1 I1 I1 safe se1 ->
   backward_simulation cc cc L1 L2 ->
-  module_safe L2 I2 I2 safe se2.
+  module_safe_se L2 I2 I2 safe se2.
 Proof.
-  (** Test2  *)
-  intros MSENV SAFE [BSIM].
-  destruct BSIM as [index order match_states SKEL PROP WF].
-  red. intros w2 VSE2 SINV2.
-  (* set (safe' (l: lts li2 li2 (state L2)) s := *)
-  (*        exists w1: inv_world I1, *)
-  (*          safe l s /\ *)
-  (*          symtbl_inv I1 w1 se1 /\ *)
-  (*          forall r1, *)
-  (*            reply_inv I1 w1 r1 -> *)
-  (*            exists r2, reply_inv I2 w2 r2). *)
+  (* (** Test2  *) *)
+  (* intros MSENV SAFE [BSIM]. *)
+  (* destruct BSIM as [index order match_states SKEL PROP WF]. *)
+  (* red. intros w2 VSE2 SINV2. *)
+  (* (* set (safe' (l: lts li2 li2 (state L2)) s := *) *)
+  (* (*        exists w1: inv_world I1, *) *)
+  (* (*          safe l s /\ *) *)
+  (* (*          symtbl_inv I1 w1 se1 /\ *) *)
+  (* (*          forall r1, *) *)
+  (* (*            reply_inv I1 w1 r1 -> *) *)
+  (* (*            exists r2, reply_inv I2 w2 r2). *) *)
 
-  (* cut (lts_safe se2 (L2 se2) I2 I2 safe' w2). *)
-  split.
-  - admit.
-  (* initial_safe *)
-  - intros q2 VQ2 QINV2.
-    destruct (inv_initial _ _ _ BSIM_INV w2 se1 se2 ccw q2 SINV2 MSENV QINV2) as (w1 & q1 & SINV1 & QINV1 & MQ).
-    assert (VSE1: Genv.valid_for (skel L1) se1).
-    (** TODO: we need the invert of match_senv_valid_for  *)
-    admit.
-    assert (VQ1: valid_query (L1 se1) q1 = true).
-    { erewrite <- bsim_match_valid_query. eauto.
-      eapply PROP. eauto.
-      auto. auto. }
-    edestruct (initial_safe _ _ _ _ _ _ (SAFE w1 VSE1 SINV1) q1 VQ1 QINV1) as ((s1 & INIT1) & INIT1'). 
-    edestruct @bsim_match_initial_states as [EXIST MATCH]; eauto.
-    split.
-    + eapply EXIST. eauto.
-    + intros s2 INIT2.
-      (** use bsim_progress *)
-      exploit MATCH; eauto.
-      intros (s1' & INIT1'' & (idx & MST)).
-      (* show s1' is safe *)
-      exploit INIT1'. eapply INIT1''. intros SAFES1'.
-      (** TODO: use safe s1' and step_safe to prove smallstep.safe s1' *)
-      eapply bsim_progress; eauto.
-      admit.
-  - intros s2 q2 REACH2 EXTERN2.
-    (** TODO: how to prove there is a reachable state s1 and s1 simulates s2*)
-    assert (A: exists s1 idx, reachable (L1 se1) s1 /\ match_states se1 se2 ccw idx s1 s2).
-    admit.
-    destruct A as (s1 & idx & REACH1 & MST).
+  (* (* cut (lts_safe se2 (L2 se2) I2 I2 safe' w2). *) *)
+  (* split. *)
+  (* - admit. *)
+  (* (* initial_safe *) *)
+  (* - intros q2 VQ2 QINV2. *)
+  (*   destruct (inv_initial _ _ _ BSIM_INV w2 se1 se2 ccw q2 SINV2 MSENV QINV2) as (w1 & q1 & SINV1 & QINV1 & MQ). *)
+  (*   assert (VSE1: Genv.valid_for (skel L1) se1). *)
+  (*   (** TODO: we need the invert of match_senv_valid_for  *) *)
+  (*   admit. *)
+  (*   assert (VQ1: valid_query (L1 se1) q1 = true). *)
+  (*   { erewrite <- bsim_match_valid_query. eauto. *)
+  (*     eapply PROP. eauto. *)
+  (*     auto. auto. } *)
+  (*   edestruct (initial_safe _ _ _ _ _ _ (SAFE w1 VSE1 SINV1) q1 VQ1 QINV1) as ((s1 & INIT1) & INIT1').  *)
+  (*   edestruct @bsim_match_initial_states as [EXIST MATCH]; eauto. *)
+  (*   split. *)
+  (*   + eapply EXIST. eauto. *)
+  (*   + intros s2 INIT2. *)
+  (*     (** use bsim_progress *) *)
+  (*     exploit MATCH; eauto. *)
+  (*     intros (s1' & INIT1'' & (idx & MST)). *)
+  (*     (* show s1' is safe *) *)
+  (*     exploit INIT1'. eapply INIT1''. intros SAFES1'. *)
+  (*     (** TODO: use safe s1' and step_safe to prove smallstep.safe s1' *) *)
+  (*     eapply bsim_progress; eauto. *)
+  (*     admit. *)
+  (* - intros s2 q2 REACH2 EXTERN2. *)
+  (*   (** TODO: how to prove there is a reachable state s1 and s1 simulates s2*) *)
+  (*   assert (A: exists s1 idx, reachable (L1 se1) s1 /\ match_states se1 se2 ccw idx s1 s2). *)
+  (*   admit. *)
+  (*   destruct A as (s1 & idx & REACH1 & MST). *)
     
     
   (** Test1  *)
